Made wfsystem require all multiequations to be well-formed, and the left-hand-sides must together contain all the variables. Also added some rewrites for FINITE and wfm implications of wfsystem.

hol/multiequation_systemScript.sml
@@ -1,20 +1,53 @@
-open HolKernel boolLib bossLib Parse multiequationTheory
+open HolKernel boolLib bossLib Parse multiequationTheory lcsymtacs
 
 val _ = new_theory "multiequation_system"
 
 val _ = type_abbrev("system", ``:('a,'b) multiequation list # ('a,'b) multiequation set``)
 
 val meqs_of_def = Define`
-  meqs_of (t,u) = set t ∪ u`;
+  meqs_of (sys:('a,'b) system) = set (FST sys) ∪ (SND sys)`;
+
+val meqs_of_pair_rewrite = Q.store_thm(
+"meqs_of_pair_rewrite",
+`meqs_of (t,u) = set t ∪ u`,
+srw_tac [][meqs_of_def]);
 
 val wfsystem_def = Define`
   wfsystem (t,u) =
     FINITE u ∧
+    RES_FORALL (meqs_of (t,u)) wfm ∧
+    BIGUNION (IMAGE vars (BIGUNION (IMAGE (SET_OF_BAG o SND) (meqs_of (t,u))))) ⊆ BIGUNION (IMAGE FST (meqs_of (t,u))) ∧
     pairwise (RC (inv_image DISJOINT FST)) (meqs_of (t,u)) ∧
-    (∀meq. MEM meq t ⇒ FINITE_BAG (SND meq) ∧ BAG_CARD (SND meq) ≤ 1) ∧
+    (∀meq. MEM meq t ⇒ BAG_CARD (SND meq) ≤ 1) ∧
     (∀i tm. i < LENGTH t ∧
             ((∃j. tm <: (SND (EL j t)) ∧ i < j ∧ j < LENGTH t) ∨
              tm ∈ BIGUNION (IMAGE (SET_OF_BAG o SND) u))
             ⇒ DISJOINT (FST (EL i t)) (vars tm))`;
+
+val wfsystem_FINITE = Q.store_thm(
+"wfsystem_FINITE",
+`wfsystem sys ⇒ FINITE (SND sys)`,
+Cases_on `sys` >> srw_tac [][wfsystem_def]);
+val _ = export_rewrites["wfsystem_FINITE"];
+
+val wfsystem_FINITE_pair = Q.store_thm(
+"wfsystem_FINITE_pair",
+`wfsystem (t,u) ⇒ FINITE u`,
+srw_tac [][wfsystem_def]);
+val _ = export_rewrites["wfsystem_FINITE_pair"];
+
+val wfsystem_wfm = Q.store_thm(
+"wfsystem_wfm",
+`(wfsystem sys ∧ meq ∈ SND sys ⇒ wfm meq) ∧
+ (wfsystem sys ∧ MEM meq (FST sys) ⇒ wfm meq)`,
+Cases_on `sys` >> srw_tac [][wfsystem_def,meqs_of_def]);
+val _ = export_rewrites["wfsystem_wfm"];
+
+val wfsystem_wfm_pair = Q.store_thm(
+"wfsystem_wfm_pair",
+`(wfsystem (t,u) ∧ meq ∈ u ⇒ wfm meq) ∧
+ (wfsystem (t,u) ∧ MEM meq t ⇒ wfm meq)`,
+srw_tac [][wfsystem_def,meqs_of_def]);
+val _ = export_rewrites["wfsystem_wfm_pair"];
 
 val _ = export_theory ()
